\newcommand{\ppplus}[0]{\textrm{plus}}
\irule
  {Abs}
  {
    \irule
      {Abs}
      {
        \inferrule*[right=(App)]
          {
            \inferrule*[right=(Var), rightskip=4em]
              { }
              {Γ^0, x:τ_1, y:τ_2 ⊢ y}
            \\
            \inferrule*[right=(App),vdots=4em,leftskip=5em,rightskip=5em]
              {
                \inferrule*[right=(Var), rightskip=6em]
                  { }
                  {Γ^0, x:τ_1, y:τ_2 ⊢ \ppplus}
                \\
                \inferrule*[right=(App),vdots=3em,leftskip=5em,rightskip=3em]
                  {
                    \inferrule*[right=(App), vdots=4em, rightskip=5em]
                      {
                        \inferrule*[right=(Var), rightskip=4em]
                          { }
                          {Γ^0, x:τ_1, y:τ_2 ⊢ \ppplus }
                        \\
                        \inferrule*[right=(Proj-G), vdots=3em, leftskip=4em]
                          {
                            \irule
                              {Var}
                              { }
                              {Γ^0, x:τ_1, y:τ_2 ⊢ x}
                          }
                          {Γ^0, x:τ_1, y:τ_2 ⊢ \textrm{fst} x}
                      }
                      {Γ^0, x:τ_1, y:τ_2 ⊢ \ppplus (\textrm{fst} x) }
                    \\
                    \inferrule*[right=(Proj-D), leftskip=5em, rightskip=4em]
                      {
                        \irule
                          {Var}
                          { }
                          {Γ^0, x:τ_1, y:τ_2 ⊢ x}
                      }
                      {Γ^0, x:τ_1, y:τ_2 ⊢ \textrm{snd} x}
                  }
                  {Γ^0, x:τ_1, y:τ_2 ⊢ \ppplus (\textrm{fst} x) (\textrm{snd} x) }
              }
              {Γ^0, x:τ_1, y:τ_2 ⊢ \ppplus (\ppplus (\textrm{fst} x) (\textrm{snd} x)) }
          }
          {Γ^0, x:τ_1, y:τ_2 ⊢ \ppplus (\ppplus (\textrm{fst} x) (\textrm{snd} x)) y }
      }
      {Γ^0, x:τ_1 ⊢ λy. \ppplus (\ppplus (\textrm{fst} x) (\textrm{snd} x)) y }
  }
  {Γ^0 ⊢ λx.λy. \ppplus (\ppplus (\textrm{fst} x) (\textrm{snd} x)) y }
